src/NonlinearArithmetic/DivMod.dfy
@@ -1,16 +1,17 @@
 // RUN: %dafny /compile:0 /noNLarith "%s" > "%t"
 // RUN: %diff "%s.expect" "%t"
 
-/***********************************************************************************
+/*******************************************************************************
 *  Original: Copyright (c) Microsoft Corporation
 *  SPDX-License-Identifier: MIT
 *  
 *  Modifications and Extensions: Copyright by the contributors to the Dafny Project
 *  SPDX-License-Identifier: MIT 
-************************************************************************************/
+*******************************************************************************/
 
-/* Every lemma comes in 2 forms: 'LemmaProperty' and 'LemmaPropertyAuto'. The former takes arguments and may 
-be more stable and less reliant on Z3 heuristics. The latter includes automation and its use requires less effort */
+/* Every lemma comes in 2 forms: 'LemmaProperty' and 'LemmaPropertyAuto'. The
+former takes arguments and may be more stable and less reliant on Z3
+heuristics. The latter includes automation and its use requires less effort */
 
 include "Internals/DivInternalsNonlinear.dfy"
 include "Internals/DivInternals.dfy"
@@ -26,9 +27,9 @@ module DivMod {
   import opened Mul
   import opened GeneralInternals
 
-  /**************************************************************************************************
+  /*****************************************************************************
   * Division:
-  **************************************************************************************************/
+  *****************************************************************************/
 
   /* the common syntax of division gives the same quotient as performing division through recursion */
   lemma LemmaDivIsDivRecursive(x: int, d: int)
@@ -926,9 +927,9 @@ module DivMod {
   }
 
 
-/*********************************************************************************************************
+/*******************************************************************************
 * Modulus:
-**********************************************************************************************************/
+*******************************************************************************/
  
   /* the common syntax of the modulus operation results in the same remainder as recursively
   calculating the modulus */
