src/NonlinearArithmetic/Internals/ModInternals.dfy
@@ -1,13 +1,13 @@
 // RUN: %dafny /compile:0 /noNLarith "%s" > "%t"
 // RUN: %diff "%s.expect" "%t"
 
-/***********************************************************************************
+/*******************************************************************************
 *  Original: Copyright (c) Microsoft Corporation
 *  SPDX-License-Identifier: MIT
 *  
 *  Modifications and Extensions: Copyright by the contributors to the Dafny Project
 *  SPDX-License-Identifier: MIT 
-************************************************************************************/
+*******************************************************************************/
 
 /* lemmas and functions in this file are used in the proofs in DivMod.dfy */
 
